learning tactics, also fix translation

src/Pipit.System.ExpX.fst
@@ -57,17 +57,17 @@ let rec oracle_of_exp (e: exp): Type =
 let osystem (input: Type) (oracle: Type) (state: Type) (result: Type) = system (input * oracle) state result
 
 (* A system we get from translating an expression *)
-let xsystem (e: exp) (vars: nat { wf e vars }) = osystem (C.row vars) (oracle_of_exp e) (state_of_exp e) value
+let xsystem (e: exp) (vars: nat { wf e vars }) = osystem (values_n vars) (oracle_of_exp e) (state_of_exp e) value
 
 let osystem_input (#input #oracle: Type): osystem input oracle unit input =
   { init = (fun s -> True);
     step = (fun io s s' r -> r == (fst io)) }
 
 let osystem_index (vars: nat) (x: nat { x < vars }):
-       osystem (C.row vars) unit unit value =
+       osystem (values_n vars) unit unit value =
   { init = (fun _ -> True);
     step = (fun io s s' r ->
-      r == C.row_index (fst io) x)
+      r == values_index vars x (fst io))
   }
 
 let osystem_map2 (#input #oracle1 #oracle2 #state1 #state2 #value1 #value2 #result: Type) (f: value1 -> value2 -> result)
@@ -100,9 +100,10 @@ let osystem_then (#input #oracle1 #oracle2 #state1 #state2 #v: Type)
     step = (fun io s s' r ->
      let i = fst io in
      let o = snd io in
-     if (fst s)
-     then t1.init o.then_s1 /\ t1.step (i, o.then_o1) o.then_s1 o.then_s1' r /\ t2.step (i, o.then_o2) (snd s) (snd s') o.then_r2
-     else fst s = false /\ t2.step (i, o.then_o2) (snd s) (snd s') r)
+     not (fst s') /\ t2.step (i, o.then_o2) (snd s) (snd s') o.then_r2 /\
+      (if fst s
+      then t1.init o.then_s1 /\ t1.step (i, o.then_o1) o.then_s1 o.then_s1' r
+      else r == o.then_r2))
   }
 
 let osystem_mu (#input #input' #oracle #state1 #v: Type)
@@ -129,177 +130,12 @@ let rec osystem_of_exp (e: exp) (vars: nat { wf e vars }):
     osystem_then (osystem_of_exp e1 vars) (osystem_of_exp e2 vars)
   | XMu e1 ->
     let t = osystem_of_exp e1 (vars + 1) in
-    osystem_mu #(C.row vars) #(C.row (vars + 1)) (fun i v -> C.row_append (C.row1 v) i) t
+    osystem_mu #(values_n vars) #(values_n (vars + 1)) (fun i v -> (v, i)) t
 
-module Ck = Pipit.Check.Example
 module T = FStar.Tactics
 
-open Pipit.System.Ind
-
-
-
-let example0_t = osystem_of_exp (Ck.example0_ok Ck.x0) 1
-
-// let example0_ok_base (): Lemma (ensures base_case' example0_t) =
-
-//   assert (base_case' example0_t) by (
-//     // T.compute ();
-//     // T.simpl ();
-//     // let _ = T.forall_intro_as "x" in
-//     // let _ = T.forall_intros () in
-//     T.norm [delta_attr [`%unfold_attr]];
-//     // T.whnf ();
-//     // T.unfold_def (`osystem_of_exp);
-//     // T.l_revert ();
-//     // T.revert ();
-//     // T.implies_intro ();
-//     // T.forall_intro ();
-//     T.compute ()
-//   );
-
-//   ()
-
-// let example0_ok_step (): Lemma (ensures step_case' example0_t) =
-//   assert (step_case' example0_t) by (
-//     // T.unfold_def (`example0_t);
-//     // T.norm [delta_attr [`%osystem_of_exp; `%wf]];
-//     // T.unfold_def (`osystem_of_exp);
-//     // let _ = T.forall_intros () in
-//     T.compute ());
-//   ()
-
-// let example1_t = osystem_of_exp (Ck.example1_bad Ck.x0) 1
-
-// let example1_nok_base (): Lemma (ensures base_case' example1_t) =
-//   assert (base_case' example1_t) by (T.compute ());
-//   ()
-
-// // this is not true, so we can't prove it
-// [@@expect_failure]
-// let example1_nok_step (): Lemma (ensures step_case' example1_t) =
-//   assert (step_case' example1_t) by (T.compute ());
-//   ()
-
-
-// // always a => always (always a)
-// let example_GA_GGA =
-//   osystem_of_exp (
-//     let open Ck in
-//     let a = x0 in
-//     sofar a => sofar (sofar a))
-//     1
-
-// let example_GA_GGA_ok (): unit =
-//   assert (base_case' example_GA_GGA) by (T.compute ());
-//   assert (step_case' example_GA_GGA) by (T.compute ());
-//   ()
-
-// // sometimes a => not (always (not a))
-// let example_F_def =
-//   osystem_of_exp (
-//     let open Ck in
-//     let a = x0 in
-//     once a => Ck.not (sofar (Ck.not a)))
-//     1
-
-// let example_F_def_ok (): unit =
-//   assert (base_case' example_F_def) by (T.compute ());
-//   assert (step_case' example_F_def) by (T.compute ());
-//   ()
-
-// // always a /\ always (a => b) => always b
-// let example_GA_GAB__GB =
-//   osystem_of_exp (
-//     let open Ck in
-//     let a = x0 in
-//     let b = x1 in
-//     (sofar a /\ sofar (a => b)) => sofar b)
-//     2
-
-// let example_GA_GAB_GB_ok (): unit =
-//   assert (base_case' example_GA_GAB__GB) by (T.compute ());
-//   assert (step_case' example_GA_GAB__GB) by (T.compute ());
-//   ()
-
-let example_FA_GAB__FB =
-  osystem_of_exp (
-    let open Ck in
-    let a = x0 in
-    let b = x1 in
-    (sofar (a => b)) => (once a => once b))
-    2
 
 let tac_nbe (): T.Tac unit = T.norm [primops; iota; delta; zeta; nbe]
-
-let tac_destruct (t: T.term): T.Tac unit =
-  T.print ("destructing " ^ T.term_to_string t);
-    T.destruct t;
-    // TODO false_elim if case not same as branch constructor
-    T.iterAll (fun () ->
-      let bs = T.repeat T.intro in
-      match bs with
-      | [] -> ()
-      | _ :: _ ->
-        let b = List.Tot.last bs in
-        T.print ("case with " ^ T.binder_to_string b ^ " of type " ^ T.term_to_string (T.type_of_binder b));
-        T.rewrite_all_context_equalities bs;
-        // T.grewrite_eq b;
-        T.norm [iota])
-
-let tac_destruct_match1 (t: T.term): T.Tac bool =
-  match T.inspect_unascribe t with
-  // TODO check that branch is not just `_`
-  | T.Tv_Match scrut _ [branch1] ->
-    let simple = match scrut with
-      | T.Tv_Uvar _ _ | T.Tv_Var _ | T.Tv_BVar _ | T.Tv_FVar _ -> true
-      | _ -> false
-    in
-    if simple then
-    begin
-      tac_destruct scrut;
-      true
-    end
-    else
-      false
-  | _ -> false
-
-let tac_destruct_term (t: T.term): T.Tac bool =
-  let rec tm (t: T.term): T.Tac bool = match T.inspect_unascribe t with
-    | T.Tv_Match sc _ brs ->
-      if tac_destruct_match1 t
-      then true
-      else begin
-        if tm sc
-        then true
-        else T.fold_left (fun acc (_, b) -> if acc then true else tm b) false brs
-      end
-    | T.Tv_Abs x t ->
-      tm t
-    | T.Tv_App f (t, _) ->
-      if tm f
-      then true
-      else tm t
-    | T.Tv_Let _ _ _ def body ->
-      if tm def
-      then true
-      else tm body
-    | _ -> false
-  in tm t
-
-let rec tac_destructor' (gas: nat): T.Tac unit =
-  if gas > 0
-  then
-    let bs = T.cur_binders () in
-    let acc = T.fold_left (fun acc b -> if acc then true else tac_destruct_term (T.type_of_binder b)) false bs in
-    if acc then tac_destructor' (gas - 1)
-
-let tac_destructor (): T.Tac unit =
-
-  tac_destructor' 10
-
-
-// let destruct_by_type (): T.Tac unit =
-//   let bs =
 
 let rec type_is_product (ty: T.typ): T.Tac bool =
   match T.inspect_unascribe ty with
@@ -333,8 +169,7 @@ let type_is_unit (ty: T.typ): T.Tac bool =
   | _ ->
     false
 
-
-let rec tac_product_go (bs: list T.binder): T.Tac unit = match bs with
+let rec tac_products (bs: list T.binder): T.Tac unit = match bs with
  | [] -> ()
  | b :: bs ->
    let open T in
@@ -347,63 +182,51 @@ let rec tac_product_go (bs: list T.binder): T.Tac unit = match bs with
     let bs' = T.repeat T.intro in
     T.rewrite_all_context_equalities bs';
     T.norm [iota];
-    // TODO clear b if possible
     let _ = T.trytac (fun () ->
       match List.Tot.rev bs' with
-      | breq :: _ ->
-        T.print ("clear " ^ T.binder_to_string breq);
-        clear breq; clear b
+      | breq :: _ -> clear breq; clear b
       | _ -> clear b
     ) in
-    tac_product_go (bs' @ bs)
+    tac_products (bs' @ bs)
    end
    else begin
     (try
       if type_is_unit ty then clear b
     with
       | _ -> ());
-    tac_product_go bs
+    tac_products bs
     end
 
-let tac_product (): T.Tac unit =
+let tac_products_all (): T.Tac unit =
   let bs = T.cur_binders () in
-  tac_product_go bs
+  tac_products bs
 
+(* Tactic for proving base case *)
+let tac_base (): T.Tac unit =
+  // Compute to simplify state_of_exp and osystem_of_exp as much as possible
+  tac_nbe ();
+  // Introduce the input, state and result quantifiers
+  let i  = T.forall_intro () in
+  let s  = T.forall_intro () in
+  let s' = T.forall_intro () in
+  let r = T.forall_intro () in
+  // Tease apart the nested tuples in the states etc
+  tac_products [i; s; s'; r];
+  // Pulling apart the states might expose a little more reduction, so take it
+  tac_nbe ()
 
-let example0_ok_baseX (): Lemma (ensures base_case' example0_t) =
+(* Tactic for proving step case *)
+let tac_step (): T.Tac unit =
+  tac_nbe ();
+  let i0  = T.forall_intro () in
+  let i1  = T.forall_intro () in
+  let s0 = T.forall_intro () in
+  let s1 = T.forall_intro () in
+  let s2 = T.forall_intro () in
+  let r0 = T.forall_intro () in
+  let r1 = T.forall_intro () in
+  // Tease apart the nested tuples in the states etc
+  tac_products [i0; i1; s0; s1; s2; r0; r1];
+  // Pulling apart the states might expose a little more reduction, so take it
+  tac_nbe ()
 
-  assert (base_case' example0_t) by (
-    tac_nbe ();
-    let i  = T.forall_intro () in
-    let s  = T.forall_intro () in
-    let s' = T.forall_intro () in
-    let r = T.forall_intro () in
-    tac_product ();
-    () // T.dump "ok"
-  );
-
-  ()
-
-// this seems like it should be true. why can't prove?
-let example_GA_GAB_FB_ok (): unit =
-  // assert (base_case' example_FA_GAB__FB) by (T.compute ()); // ; T.dump "base GA_FAB_FB");
-  // assume (step_case' example_FA_GAB__FB);
-  assert (step_case' example_FA_GAB__FB) by
-    (
-    tac_nbe ();
-    let i0  = T.forall_intro () in
-    let i1  = T.forall_intro () in
-    let s0 = T.forall_intro () in
-    let s2 = T.forall_intro () in
-    let s2 = T.forall_intro () in
-    let r0 = T.forall_intro () in
-    let r1 = T.forall_intro () in
-    tac_product ();
-    // tac_destruct i;
-    // tac_destruct s;
-    // tac_destruct s';
-    // tac_destructor ();
-    T.dump "ok");
-  ()
-
-// // T.destruct
