src/Pipit.Check.Example.TacX.fst
@@ -1,0 +1,101 @@
+module Pipit.Check.Example.TacX
+
+open Pipit.System.Base
+open Pipit.System.Ind
+open Pipit.System.ExpX
+
+module T = FStar.Tactics
+
+
+module Ck = Pipit.Check.Example
+
+// always a => sometimes a
+let example_GA_FA =
+  osystem_of_exp (
+    let open Ck in
+    sofar x0 => once x0) 1
+
+let example_GA_FA_base (): Lemma (ensures base_case' example_GA_FA) =
+  assert (base_case' example_GA_FA) by tac_nbe ()
+
+let example_GA_FA_step (): Lemma (ensures step_case' example_GA_FA) =
+  assert (step_case' example_GA_FA) by tac_nbe ()
+
+// sometimes a => always a (not true)
+let example_FA_GA =
+  osystem_of_exp (
+    let open Ck in
+    once x0 => sofar x0) 1
+
+let example_FA_GA_base (): Lemma (ensures base_case' example_FA_GA) =
+  assert (base_case' example_FA_GA) by tac_base ()
+
+// this is not true so we can't prove it, but unfortunately we can't automatically disprove it
+[@@expect_failure]
+let example_FA_GA_step (): Lemma (ensures step_case' example_FA_GA) =
+  assert (step_case' example_FA_GA) by tac_step ()
+
+// always a => always (always a)
+let example_GA_GGA =
+  osystem_of_exp (
+    let open Ck in
+    let a = x0 in
+    sofar a => sofar (sofar a))
+    1
+
+let example_GA_GGA_ok (): unit =
+  assert (base_case' example_GA_GGA) by tac_nbe ();
+  assert (step_case' example_GA_GGA) by tac_nbe ()
+
+// sometimes a => not (always (not a))
+let example_FA_nGnA =
+  osystem_of_exp (
+    let open Ck in
+    let a = x0 in
+    once a => Ck.not (sofar (Ck.not a)))
+    1
+
+let example_FA_nGnA_ok (): unit =
+  assert (base_case' example_FA_nGnA) by tac_nbe ();
+  assert (step_case' example_FA_nGnA) by tac_nbe ()
+
+// always a /\ always (a => b) => always b
+let example_GA_GAB__GB =
+  osystem_of_exp (
+    let open Ck in
+    let a = x0 in
+    let b = x1 in
+    (sofar a /\ sofar (a => b)) => sofar b)
+    2
+
+let example_GA_GAB_GB_ok (): unit =
+  assert (base_case' example_GA_GAB__GB) by tac_nbe ();
+  assert (step_case' example_GA_GAB__GB) by tac_nbe ();
+  ()
+
+let example_FA_GAB__FB =
+  osystem_of_exp (
+    let open Ck in
+    let a = x0 in
+    let b = x1 in
+    (sofar (a => b)) => (once a => once b))
+    2
+
+let example_GA_GAB_FB_ok (): Lemma (ensures base_case' example_FA_GAB__FB) =
+  assert (base_case' example_FA_GAB__FB) by tac_nbe ();
+  assert (step_case' example_FA_GAB__FB) by tac_nbe ()
+
+
+let example_requires_invariant =
+  osystem_of_exp (
+    let open Ck in
+    let a = x0 in
+    let b = x1 in
+    let c = x2 in
+    (once a => (once a => once b) => (once b => once c) => once c))
+    3
+
+[@@expect_failure]
+let example_requires_invariant' (): Lemma (ensures base_case' example_requires_invariant) =
+  assert (base_case' example_requires_invariant) by (tac_base (); T.dump "asdf")
+  // assert (step_case' example_requires_invariant) by tac_nbe ()
